theories/DiophantineConstraints/Reductions/H10UC_SAT_to_H10UPC_SAT.v
@@ -6,19 +6,20 @@
     Uniform Diophantine Pair Constraint Solvability (H10UPC_SAT)
 *)
 
-Require Import List Lia.
+Require Import List Lia Cantor.
 Import ListNotations.
 
+Require Import ssreflect ssrbool ssrfun.
+
 Require Import Undecidability.DiophantineConstraints.H10C.
-Require Import Undecidability.DiophantineConstraints.H10UPC.
 
 Set Default Proof Using "Type".
 Set Default Goal Selector "!".
 
-  (* Uniform Diophantine pairs constraints are of shape:  
-      (x, y) # (1 + x + y, (y²+y)/2)
-     Uniform Diophantine constraints are of shape:
-      1 + x + y * y = z
+(* Uniform Diophantine pairs constraints are of shape:  
+    (x, y) # (1 + x + y, (y²+y)/2)
+   Uniform Diophantine constraints are of shape:
+    1 + x + y * y = z
 
   Idea: We represent 1+x+y²=z as such: 
   (where a, b, c, t1, t2 are new variables):
@@ -28,158 +29,99 @@ Set Default Goal Selector "!".
   x+c+1 = z (-> z = 1+x+y²)
 
   This yields these constraints 
-  (3 suffice (!) since we can merge constraint 1 and 3 
-     into the same pair-constraint)
   (a,a) # (b,t1)
   (c,y) # (b,a)
   (c,x) # (z,t2)
 
   We use the following renaming scheme:
-  <x,v0> = x                          (used for x,y,z)
-  <x,v1> = (x²+x)/2                   (used for a (with y), t2 (with x))
-  <x,v2> = x²+x+1                     (used for b (with y))
-  <x,v3> = x²                         (used for c (with y))
-  <x,v4> = (k²+k)/2 where k=(x²+x)/2  (used for t1 (with y))
-
-  *)
+  <x,0> = x                          (used for x,y,z)
+  <x,1> = (x²+x)/2                   (used for a (with y), t2 (with x))
+  <x,2> = x²+x+1                     (used for b (with y))
+  <x,3> = x²                         (used for c (with y))
+  <x,4> = (k²+k)/2 where k=(x²+x)/2  (used for t1 (with y))
+*)
 
 Module Argument.
 
-Definition c2_full (x:nat) : {y:nat | x * S x = y+y}.
+Definition c2_full (x: nat) : { y:nat | y + y = x * S x}.
 Proof.
-  induction x as [|x [y' IH]].
-  - exists 0. lia.
-  - exists (y'+x+1). nia.
-Defined.
-
-Definition c2 (x:nat) := match (c2_full x) with exist _ y _ => y end.
-
-Definition c2_descr (x:nat) : x * S x = c2 x + c2 x.
-Proof.
-unfold c2. now destruct (c2_full x).
-Qed. 
-
-(* We generate 5 new variables for each variable. 
-   The following type encodes the choices *)
-Inductive fin5 := v0 | v1 | v2 | v3 | v4.
-Definition fin2nat y := match y with v0=>0|v1=>1|v2=>2|v3=>3|v4=>4 end.
-Definition encode5 '(x,y) := x*5+fin2nat y.
-Fixpoint decode5 k := match k with 
-          0 => (0,v0) 
-        | 1 => (0,v1) 
-        | 2 => (0,v2) 
-        | 3 => (0,v3) 
-        | 4 => (0,v4) 
-        | S(S(S(S(S kk)))) => let '(x,y) := decode5 kk in (S x,y) end.
-
-Lemma decode_encode x y : decode5 (encode5 (x,y)) = (x,y).
-Proof.
-  induction x as [|x IH].
-  - now destruct y.
-  - cbn. destruct (decode5 (x*5+fin2nat y)) as [x' y'] eqn:Heq. 
-    change (x*5+fin2nat y) with (encode5 (x,y)) in Heq. congruence.
+  elim: x; first by exists 0.
+  move=> x [y Hy]. exists (y+x+1). nia.
 Qed.
 
-Opaque decode5 encode5.
+#[local] Notation c2 x := (sval (c2_full x)).
+#[local] Notation c2_spec x := (svalP (c2_full x)).
+
+(* fresh variable space *)
+Notation var x t := (Cantor.to_nat (x, t)).
+Opaque Cantor.to_nat Cantor.of_nat.
 
 Section Reduction.
-Definition rename x := encode5 (x,v0).
-Definition newvar x t := encode5 (x,t).
+(* The instance of h10uc (which we are reducing from) *)
+Context (ucs: list h10uc).
 
-Definition h10uc_to_h10upc_single : h10uc -> list h10upc := (fun '(x,y,z) => 
-  let '(a,b,c,t1,t2) := 
-            (newvar y v1,newvar y v2,newvar y v3,newvar y v4,newvar x v1) in
-  let '(x,y,z) := (rename x,rename y,rename z) in
-  [((a,a),(b,t1)); ((c,y),(b,a)); ((c,x),(z,t2))]).
+Definition h10uc_to_h10upcs (c : h10uc) : list h10upc := 
+  let '(x, y, z) := c in
+  let '(a, b, c, t1, t2) := (var y 1, var y 2, var y 3, var y 4, var x 1) in
+  let '(x, y, z) := (var x 0, var y 0, var z 0) in
+    [((a, a), (b, t1)); ((c, y), (b, a)); ((c, x), (z, t2))].
 
-Definition h10uc_to_h10upc := flat_map h10uc_to_h10upc_single.
-
-End Reduction.
+Definition upcs := flat_map h10uc_to_h10upcs ucs.
 
 Section Transport.
-(* The instance of h10uc (which we are reducing from) *)
-Context (cs: list h10uc).
 (* The solution to cs *)
-Context (φ: nat -> nat). 
-(* Proof that it actually is a solution *)
-Context (Hφ : forall c, In c cs -> h10uc_sem φ c). 
+Context (φ: nat -> nat).
+(* Proof that φ solves ucs *)
+Context (Hφ : forall c, In c ucs -> h10uc_sem φ c). 
 
-Definition φ' (xn:nat) : nat := match decode5 xn with
-    (x,v0) => φ x
-  | (x,v1) => c2 (φ x)
-  | (x,v2) => φ x * φ x + φ x + 1
-  | (x,v3) => φ x * φ x
-  | (x,v4) => c2 (c2 (φ x)) end.
+Definition φ' (xn: nat) : nat :=
+  match Cantor.of_nat xn with
+  | (x, 0) => φ x
+  | (x, 1) => c2 (φ x)
+  | (x, 2) => φ x * φ x + φ x + 1
+  | (x, 3) => φ x * φ x
+  | (x, 4) => c2 (c2 (φ x))
+  | _ => 0
+  end.
 
-Lemma transport_single c : h10uc_sem φ c -> 
-          forall cc, In cc (h10uc_to_h10upc_single c) -> h10upc_sem φ' cc.
-Proof.
-  intros H cc. destruct c as [[x y] z]. intros [c'|[c'|[c'|[]]]]; subst. 
-  all:unfold rename, newvar, φ'; cbn. all: rewrite !decode_encode. all: split.
-  - rewrite <- c2_descr. lia. 
-  - apply c2_descr.
-  - lia.
-  - apply c2_descr. 
-  - cbn in H. nia. 
-  - apply c2_descr.
-Qed.
-
-Lemma transport : forall c, In c (h10uc_to_h10upc cs) -> h10upc_sem φ' c.
+Lemma transport : forall c, In c upcs -> h10upc_sem φ' c.
 Proof using Hφ.
-  intros c H%(in_flat_map_Exists h10uc_to_h10upc_single c cs).
-  induction cs as [|cc cs' IHcs].
-  - now apply Exists_nil in H.
-  - apply Exists_cons in H as [Hl|Hr].
-    + apply (transport_single cc).
-      * apply Hφ. now left.
-      * easy.
-    + apply IHcs.
-      * intros c' Hc'. apply Hφ. now right.
-      * easy.
+  apply /Forall_forall /Forall_flat_map.
+  move: Hφ => /Forall_forall.
+  apply: Forall_impl => - [[x y] z] /= ?.
+  constructor; [|constructor; [|constructor]]; last done.
+  all: rewrite /φ' /= ?Cantor.cancel_of_to ?(c2_spec _); lia.
 Qed.
 
 End Transport.
 
 Section InverseTransport.
-(* The instance of h10uc (which we are reducing from) *)
-Context (cs: list h10uc).
- (* The solution to f(cs) (f is the reduction function) *) 
+(* The solution to f(cs) (f is the reduction function) *) 
 Context (φ': nat -> nat).
-(* Proof that it actually is a solution *)
-Context (Hφ' : forall c, In c (h10uc_to_h10upc cs) -> h10upc_sem φ' c). 
+(* Proof that φ' solves upcs *)
+Context (Hφ' : forall c, In c upcs -> h10upc_sem φ' c). 
 
-(* Lookup variables in result env *)
-Definition φ (n:nat) : nat := φ' (rename n). 
+Definition φ (n:nat) : nat := φ' (var n 0). 
 
-Lemma inverse_transport_single c : 
-      (forall cc, In cc (h10uc_to_h10upc_single c) -> h10upc_sem φ' cc) 
-       -> h10uc_sem φ c.
-Proof.
-  intros H. destruct c as [[x y] z]. cbn.
-  cbn in H.
-  assert (h10upc_sem φ' ((newvar y v1, newvar y v1), (newvar y v2, newvar y v4))) 
-    as [HC1l _] by (apply H; tauto).
-  assert (h10upc_sem φ' ((newvar y v3, rename y), (newvar y v2, newvar y v1))) 
-    as [HC2l HC2r] by (apply H; tauto).
-  assert (h10upc_sem φ' ((newvar y v3, rename x), (rename z, newvar x v1))) 
-    as [HC3l _] by (apply H; tauto).
-  unfold φ. nia.
-Qed.
-
-Lemma inverse_transport : forall c, In c cs -> h10uc_sem φ c.
+Lemma inverse_transport : forall c, In c ucs -> h10uc_sem φ c.
 Proof using Hφ'.
-  intros c H.
-  apply inverse_transport_single. intros cc Hcc. apply Hφ'.
-  unfold h10uc_to_h10upc. apply in_flat_map. exists c. now split.
+  apply /Forall_forall.
+  move: Hφ' => /Forall_forall /Forall_flat_map.
+  apply: Forall_impl => - [[x y] z] /=.
+  move=> /Forall_cons_iff [+] /Forall_cons_iff [+] /Forall_cons_iff [+ _].
+  rewrite /φ /=. nia.
 Qed.
 
 End InverseTransport.
+End Reduction.
 End Argument.
+
 Require Import Undecidability.Synthetic.Definitions.
 
 (** Square Diophantine Constraint Solvability many-one reduces to Uniform Diophantine Constraint Solvability *)
 Theorem reduction : H10UC_SAT ⪯ H10UPC_SAT.
-Proof. exists Argument.h10uc_to_h10upc. split.
- - intros [φ Hφ]. exists (Argument.φ' φ). now apply Argument.transport.
- - intros [φ' Hφ']. exists (Argument.φ φ'). now apply Argument.inverse_transport.
+Proof.
+  exists Argument.upcs. split.
+  - intros [φ Hφ]. exists (Argument.φ' φ). now apply Argument.transport.
+  - intros [φ' Hφ']. exists (Argument.φ φ'). now apply Argument.inverse_transport.
 Qed.
