theories/DiophantineConstraints/H10C_undec.v
@@ -1,7 +1,8 @@
 (* 
   Autor(s):
     Dominique Larchey-Wendling (1)
-    Andrej Dudenhefner (2) 
+    Andrej Dudenhefner (2)
+    Johannes Hostert (2)
   Affiliation(s):
     (1) LORIA -- CNRS
     (2) Saarland University, Saarbrücken, Germany
@@ -14,6 +15,7 @@
     Diophantine Constraint Solvability (H10C_SAT)
     Square Diophantine Constraint Solvability (H10SQC_SAT)
     Uniform Diophantine Constraint Solvability (H10UC_SAT)
+    Uniform Diophantine Pair Constraint Solvability (H10UPC_SAT)
 *)
 
 Require Import Undecidability.Synthetic.Undecidability.
@@ -22,7 +24,7 @@ Require Import Undecidability.Synthetic.ReducibilityFacts.
 Require Import Undecidability.DiophantineConstraints.H10C.
 
 From Undecidability.DiophantineConstraints.Reductions Require
-  FRACTRAN_to_H10C_SAT H10C_SAT_to_H10SQC_SAT H10SQC_SAT_to_H10UC_SAT.
+  FRACTRAN_to_H10C_SAT H10C_SAT_to_H10SQC_SAT H10SQC_SAT_to_H10UC_SAT H10UC_SAT_to_H10UPC_SAT.
 
 From Undecidability.FRACTRAN Require Import FRACTRAN FRACTRAN_undec.
 
@@ -47,4 +49,10 @@ Theorem H10UC_SAT_undec : undecidable H10UC_SAT.
 Proof.
   apply (undecidability_from_reducibility H10SQC_SAT_undec).
   exact H10SQC_SAT_to_H10UC_SAT.reduction.
+Qed.
+
+Theorem H10UPC_SAT_undec : undecidable H10UPC_SAT.
+Proof.
+  apply (undecidability_from_reducibility H10UC_SAT_undec).
+  exact H10UC_SAT_to_H10UPC_SAT.reduction.
 Qed.
